PREFIX : <https://linked.data.gov.au/def/observable-properties/>
PREFIX cs: <https://linked.data.gov.au/def/observable-properties>
PREFIX dcterms: <http://purl.org/dc/terms/>
PREFIX qk: <http://qudt.org/vocab/quantitykind/>
PREFIX prov: <http://www.w3.org/ns/prov#>
PREFIX skos: <http://www.w3.org/2004/02/skos/core#>
PREFIX xsd: <http://www.w3.org/2001/XMLSchema#>
PREFIX rdfs: <http://www.w3.org/2000/01/rdf-schema#>

qk:AmountOfSubstancePerUnitMass
    a skos:Concept ;
    skos:definition "The rate of presence of a substance within another substance"@en ;
    rdfs:isDefinedBy <http://qudt.org/vocab/quantitykind> ;
    skos:inScheme cs: ;
    skos:topConceptOf cs: ;
    skos:prefLabel "Amount Of Substance Per Unit Mass"@en ;
    skos:scopeNote "This Concept is taken from QUDT's Quantity Kinds vocabulary and acts as the top Concept of all occurrence Observable Properties" ;
    skos:historyNote "Defined by QUDT" ;
.

:amount-of-an-element
    a skos:Concept ;
    rdfs:isDefinedBy cs: ;
    skos:broader qk:AmountOfSubstancePerUnitMass ;
    skos:definition "The rate of presence of a chemical element within another substance"@en ;
    skos:inScheme cs: ;
    skos:prefLabel "Amount of an Element Per Unit Mass"@en ;
    skos:historyNote "Defined for the first time in this vocabulary" ;
.

:amount-of-an-isotope
    a skos:Concept ;
    rdfs:isDefinedBy cs: ;
    skos:broader :amount-of-an-element ;
    skos:definition "The rate of presence of a chemical isotope of an element within another substance"@en ;
    skos:inScheme cs: ;
    skos:prefLabel "Amount of an Isotope Per Unit Mass"@en ;
    skos:historyNote "Defined for the first time in this vocabulary" ;
.

:amount-of-a-compound
    a skos:Concept ;
    rdfs:isDefinedBy cs: ;
    skos:broader qk:AmountOfSubstancePerUnitMass ;
    skos:definition "The rate of presence of a chemical compound within another substance"@en ;
    skos:inScheme cs: ;
    skos:prefLabel "Amount of a Compound Per Unit Mass"@en ;
    skos:historyNote "Defined for the first time in this vocabulary" ;
.

:amount-of-bauxite
    a skos:Concept ;
    rdfs:isDefinedBy cs: ;
    skos:broader :amount-of-a-compound ;
    skos:definition "The rate of presence of the clay bauxite within another substance"@en ;
    skos:inScheme cs: ;
    skos:prefLabel "Amount of Bauxite Per Unit Mass"@en ;
    skos:historyNote "Defined for the first time in this vocabulary" ;
.

:amount-of-a-metal
    a skos:Concept ;
    rdfs:isDefinedBy cs: ;
    skos:broader :amount-of-an-element ;
    skos:definition "The rate of presence of a metallic chemical element within another substance"@en ;
    skos:inScheme cs: ;
    skos:prefLabel "Amount of a Metal Per Unit Mass"@en ;
    skos:historyNote "Defined for the first time in this vocabulary" ;
.

:amount-of-a-mineral
    a skos:Concept ;
    rdfs:isDefinedBy cs: ;
    skos:broader :amount-of-a-compound ;
    skos:definition "The rate of presence of a mineral within another substance"@en ;
    skos:inScheme cs: ;
    skos:prefLabel "Amount of a Mineral Per Unit Mass"@en ;
    skos:historyNote "Defined for the first time in this vocabulary" ;
.

:amount-of-basalt
    a skos:Concept ;
    rdfs:isDefinedBy cs: ;
    skos:broader :amount-of-a-compound ;
    skos:definition "The rate of presence of basaltic rocks within another substance"@en ;
    skos:inScheme cs: ;
    skos:prefLabel "Amount of a Basalt Per Unit Mass"@en ;
    skos:historyNote "Defined for the first time in this vocabulary" ;
.

:amount-of-gold
    a skos:Concept ;
    rdfs:isDefinedBy cs: ;
    skos:broader :amount-of-a-metal ;
    skos:definition "The rate of presence of elemental gold within another substance"@en ;
    skos:inScheme cs: ;
    skos:prefLabel "Amount of Gold Per Unit Mass"@en ;
    skos:historyNote "Defined for the first time in this vocabulary" ;
.

:amount-of-uranium
    a skos:Concept ;
    rdfs:isDefinedBy cs: ;
    skos:broader :amount-of-a-metal ;
    skos:definition "The rate of presence of elemental uranium within another substance"@en ;
    skos:inScheme cs: ;
    skos:prefLabel "Amount of Uranium Per Unit Mass"@en ;
    skos:historyNote "Defined for the first time in this vocabulary" ;
.

:amount-of-uranium-235
    a skos:Concept ;
    rdfs:isDefinedBy cs: ;
    skos:broader :amount-of-a-uranium , :amount-of-an-isotope ;
    skos:definition "The rate of presence of uranium 235 isotope within another substance"@en ;
    skos:inScheme cs: ;
    skos:prefLabel "Amount of Uranium 235 Per Unit Mass"@en ;
    skos:historyNote "Defined for the first time in this vocabulary" ;
.

:amount-of-uranium-238
    a skos:Concept ;
    rdfs:isDefinedBy cs: ;
    skos:broader :amount-of-a-uranium , :amount-of-an-isotope ;
    skos:definition "The rate of presence of uranium 238 isotope within another substance"@en ;
    skos:inScheme cs: ;
    skos:prefLabel "Amount of Uranium 238 Per Unit Mass"@en ;
    skos:historyNote "Defined for the first time in this vocabulary" ;
.

cs:
    a skos:ConceptScheme ;
    dcterms:created "2023-06-16"^^xsd:date ;
    dcterms:creator <https://linked.data.gov.au/org/gswa> ;
    dcterms:modified "2023-06-16"^^xsd:date ;
    dcterms:creator <https://orcid.org/0000-0002-8742-7730> ;
    dcterms:publisher
        <https://linked.data.gov.au/org/gsq> ,
        <https://linked.data.gov.au/org/gwa> ;
    skos:definition "Observable quality (property, characteristic) of a Feature Of Interest" ;
    skos:hasTopConcept qk:AmountOfSubstancePerUnitMass ;
    skos:prefLabel "Observable Properties"@en ;
    prov:qualifiedDerivation [
        prov:hadRole <https://linked.data.gov.au/def/vocdermods/none>
    ] ;
    skos:historyNote """This vocabulary was created as a fundamental vocabulary supporting data about the observations and measurements of phenomena.

The Sensor, Observation, Sample, and Actuator (SOSA) Ontology which is a Semantic Web implementation of the ISO's Observations & Measurement standard defines an Observable Property class and this vocabulary can be taken as defining instances of that class.""" ;
.
